completed hkdf proof

providers/evercrypt/fst/EverCrypt.HKDF.fst
@@ -16,9 +16,10 @@ open EverCrypt.Hash
 
 type alg = EverCrypt.HMAC.ha
 
+// [hashed] holds the HMAC text, 
+// of the form | tagLen a | infolen | 1 |;
+// its prefix is overwritten by HMAC at each iteration.
 
-//18-03-05 I'd rather verify a simpler implementation, closer to the spec, as outlined below. 
-//18-03-05 We could make do with fewer loop variables if it helps with C.Loops
 private val hkdf_expand_loop: 
   a       : alg -> (
   okm     : uint8_p ->
@@ -29,28 +30,25 @@ private val hkdf_expand_loop:
   hashed  : uint8_pl (tagLength (Ghost.hide a) + v infolen + 1) ->
   i       : UInt8.t {
     let a = Ghost.hide a in 
-    let count = v i in 
-    let required = v len in 
     HMAC.keysized a (length prk) /\ 
     disjoint okm prk /\
     disjoint hashed okm /\ 
     disjoint hashed prk /\
     tagLength a + v infolen + 1 + blockLength a < pow2 32 /\ (* specific to this implementation *)
     tagLength a + pow2 32 + blockLength a <= maxLength a /\
-    count < 255 /\
-    required <= (255 - count) * tagLength a } ->
+    v i < 255 /\
+    v len <= (255 - v i) * tagLength a } ->
   ST unit
   (requires fun h0 -> 
     live h0 okm /\ live h0 prk /\ live h0 hashed)
   (ensures  fun h0 r h1 -> 
-    //live h1 okm /\ 
     LowStar.Modifies.(modifies (loc_union (loc_buffer okm) (loc_buffer hashed)) h0 h1) /\ (
-    let prk = as_seq h0 prk in 
+    let prk  = as_seq h0 prk in 
     let info = as_seq h0 (gsub hashed (tagLen a) infolen) in 
     let last = if i = 0uy then Seq.empty else as_seq h0 (gsub hashed 0ul (tagLen a)) in 
-    let okm = as_seq h1 okm in 
-    okm == expand0 (Ghost.hide a) prk info (v len) (v i) last)))
+    as_seq h1 okm == expand0 (Ghost.hide a) prk info (v len) (v i) last)))
 
+//18-07-13 how to improve this proof? should we use C.loops instead? 
 #set-options "--z3rlimit 100"
 let rec hkdf_expand_loop a okm prk prklen infolen len hashed i =
   push_frame ();
@@ -61,81 +59,82 @@ let rec hkdf_expand_loop a okm prk prklen infolen len hashed i =
   let counter = offset info_counter infolen in 
   assert(disjoint tag info /\ disjoint tag counter /\ disjoint info counter);
 
-  let i' = i + 1uy in
-
   let h0 = ST.get() in  // initial state
+  let i' = i + 1uy in
   counter.(0ul) <- i';
 
   let h1 = ST.get() in // before hashing
-  FStar.Seq.(lemma_eq_intro (upd (as_seq h0 counter) 0 i') (create 1 i'));
-  assert(as_seq h1 counter == Seq.create 1 i');
+  Seq.lemma_eq_intro (as_seq h1 counter) (Seq.create 1 i');
 
-  // derive an extra tag 
+  // derive an extra hash tag 
   if i = 0uy then (
     // the first input is shorter, does not include the chaining block
     let len1 = infolen + 1ul in 
     HMAC.compute a tag prk prklen info_counter len1;
-
-    let h2 = ST.get() in 
-    ( let info1 = as_seq h1 info in 
+    ( let h2 = ST.get() in 
+      let info = as_seq h0 info in 
       let ctr1 = as_seq h1 counter in 
-      let prk1 = as_seq h1 prk in 
+      let prk  = as_seq h0 prk in 
       let tag2 = as_seq h2 tag in 
-      let text = Seq.empty @| info1 @| ctr1 in
-
+      let text = Seq.empty @| info @| ctr1  in
+      // Seq.lemma_eq_intro (as_seq h1 counter) ctr1;
       // assert(tag2 == HMAC.hmac a v_prk (as_seq h1 hashed1)); 
       Seq.lemma_eq_intro (as_seq h1 info_counter) text;
-      assert(tag2 == HMAC.hmac (Ghost.hide a) prk1 text)  ))
+      assert(tag2 == HMAC.hmac (Ghost.hide a) prk text)  ))
   else (
     HMAC.compute a tag prk prklen hashed (tlen + infolen + 1ul);
-    let h2 = ST.get() in 
-    ( let info1 = as_seq h1 info in 
+    ( let h2 = ST.get() in 
+      let info = as_seq h0 info in 
       let ctr1 = as_seq h1 counter in 
-      let prk1 = as_seq h1 prk in 
+      let prk  = as_seq h0 prk in 
       let tag1 = as_seq h1 tag in 
       let tag2 = as_seq h2 tag in 
-      let text = tag1 @| info1 @| ctr1 in
-      assert(tag2 == HMAC.hmac (Ghost.hide a) prk1 (as_seq h1 hashed)); 
+      let text = tag1 @| info @| ctr1 in
+      // assert(tag2 == HMAC.hmac (Ghost.hide a) prk (as_seq h1 hashed)); 
       Seq.lemma_eq_intro (as_seq h1 hashed) text ; 
-      assert(tag2 == HMAC.hmac (Ghost.hide a) prk1 text )
-    ));
+      assert(tag2 == HMAC.hmac (Ghost.hide a) prk text )));
 
-  // copy it to the result, and iterate if required
-  if len <= tlen then 
-    blit tag 0ul okm 0ul len
+  // copy it to the result; iterate if required
+  let h2 = ST.get() in
+  if len <= tlen then (
+    blit tag 0ul okm 0ul len;
+    ( let h3 = ST.get() in 
+      let prk  = as_seq h0 prk in 
+      let info = as_seq h0 info in 
+      let last = if i = 0uy then Seq.empty else as_seq h1 tag in 
+      let text = last @| info @| Seq.create 1 i' in 
+      let tag2 = as_seq h2 tag in 
+      let result = Seq.slice (as_seq h3 okm) 0 (v len) in 
+      // assert(tag2 == HMAC.hmac (Ghost.hide a) prk text);
+      assert(result == Seq.slice tag2 0 (v len));
+      assert(result == expand0 (Ghost.hide a) prk info (v len) (v i) last) ))
   else (
     blit tag 0ul okm 0ul tlen;
-    let len = len - tlen in 
-    let okm = sub okm tlen len in 
-    let h2 = ST.get() in 
-    hkdf_expand_loop a okm prk prklen infolen len hashed i';
-
     let h3 = ST.get() in 
-    assert(
-      let prk = as_seq h0 prk in 
-      let info = as_seq h0 (gsub hashed (tagLen a) infolen) in 
-      let last = if i' = 0uy then Seq.empty else as_seq h2 (gsub hashed 0ul (tagLen a)) in 
-      let okm = as_seq h3 okm in 
-      okm ==  expand0 (Ghost.hide a) prk info (v len) (v i') last)
-    );
-
-  // TODO complete functional correctness
-  let h3 = ST.get() in 
-  assume(
-      let prk = as_seq h0 prk in 
-      let info = as_seq h0 (gsub hashed (tagLen a) infolen) in 
-      let last = if i = 0uy then Seq.empty else as_seq h0 (gsub hashed 0ul (tagLen a)) in 
-      let okm = as_seq h3 okm in 
-      okm ==  expand0 (Ghost.hide a) prk info (v len) (v i) last);
-
+    let len' = len - tlen in 
+    let okm_tag = sub okm 0ul tlen in 
+    let okm' = offset okm tlen in 
+    hkdf_expand_loop a okm' prk prklen infolen len' hashed i';
+    ( assert(disjoint okm_tag okm');
+      let h4 = ST.get() in
+      let info = as_seq h0 info in 
+      let prk  = as_seq h0 prk in 
+      let last = if i = 0uy then Seq.empty else as_seq h1 tag in 
+      let text = last @| info @| Seq.create 1 i' in 
+      let tag2 = as_seq h2 tag in 
+      // assert(tag2 == HMAC.hmac (Ghost.hide a) prk text);
+      assert(tag2 == as_seq h4 okm_tag);
+      let okm' = as_seq h4 okm' in 
+      Seq.lemma_eq_intro (tag2 @| okm') (as_seq h4 okm);
+      assert(        okm' == expand0 (Ghost.hide a) prk info (v len') (v i') tag2);
+      assert(tag2 @| okm' == expand0 (Ghost.hide a) prk info (v len) (v i) last)
+    ));
   pop_frame()
 
-// | tagLen a | infolen | 1 | 
-  
+
 let hkdf_extract a prk salt saltlen ikm ikmlen =
     HMAC.compute a prk salt saltlen ikm ikmlen
 
-#set-options "--z3rlimit 20"
 let hkdf_expand a okm prk prklen info infolen len = 
   push_frame();
   let tlen = tagLen a in 
